Add two new generator examples and fix BST
- Add BtSorting that builds a sorted list by sorting a random list
- Add ByInsertion that builds a BST via repeated calls to `insert`
- Fixes a bounds issue with BST (Closes #14.)
- Adds some infrastructure to support the above

Basalt/Tuning/Attr.lean
@@ -16,7 +16,7 @@ generator definition:
 
 ```lean
 @[tunable]
-def genBST [Gen G] (lo hi : Nat) : G (Tree Nat) := do
+def genBST [Gen G] (lo hi : Int) : G (Tree Int) := do
   if h : lo > hi then return leaf
   else frequency [
     (1, fun _ => pure leaf),
